<h2><a href="https://leetcode.com/problems/remove-palindromic-subsequences/"><div id="big-omega-company-tags"><div id="big-omega-topbar"><div class="companyTagsContainer" style="overflow-x: scroll; flex-wrap: nowrap;"><div class="companyTagsContainer--tag" style="background-color: rgba(0, 10, 32, 0.05);"><div>Bloomberg</div><div class="companyTagsContainer--tagOccurence">2</div></div></div><div class="companyTagsContainer--chevron"><div><svg version="1.1" id="icon" xmlns="http://www.w3.org/2000/svg" xmlns:xlink="http://www.w3.org/1999/xlink" x="0px" y="0px" viewBox="0 0 32 32" fill="#4087F1" xml:space="preserve" style="width: 20px;"><polygon points="16,22 6,12 7.4,10.6 16,19.2 24.6,10.6 26,12 "></polygon><rect id="_x3C_Transparent_Rectangle_x3E_" class="st0" fill="none" width="32" height="32"></rect></svg></div></div></div></div>1332. Remove Palindromic Subsequences</a></h2><h3>Easy</h3><hr><div><p>You are given a string <code>s</code> consisting <strong>only</strong> of letters <code>'a'</code> and <code>'b'</code>. In a single step you can remove one <strong>palindromic subsequence</strong> from <code>s</code>.</p>

<p>Return <em>the <strong>minimum</strong> number of steps to make the given string empty</em>.</p>

<p>A string is a <strong>subsequence</strong> of a given string if it is generated by deleting some characters of a given string without changing its order. Note that a subsequence does <strong>not</strong> necessarily need to be contiguous.</p>

<p>A string is called <strong>palindrome</strong> if is one that reads the same backward as well as forward.</p>

<p>&nbsp;</p>
<p><strong class="example">Example 1:</strong></p>

<pre><strong>Input:</strong> s = "ababa"
<strong>Output:</strong> 1
<strong>Explanation:</strong> s is already a palindrome, so its entirety can be removed in a single step.
</pre>

<p><strong class="example">Example 2:</strong></p>

<pre><strong>Input:</strong> s = "abb"
<strong>Output:</strong> 2
<strong>Explanation:</strong> "<u>a</u>bb" -&gt; "<u>bb</u>" -&gt; "". 
Remove palindromic subsequence "a" then "bb".
</pre>

<p><strong class="example">Example 3:</strong></p>

<pre><strong>Input:</strong> s = "baabb"
<strong>Output:</strong> 2
<strong>Explanation:</strong> "<u>baa</u>b<u>b</u>" -&gt; "<u>b</u>" -&gt; "". 
Remove palindromic subsequence "baab" then "b".
</pre>

<p>&nbsp;</p>
<p><strong>Constraints:</strong></p>

<ul>
	<li><code>1 &lt;= s.length &lt;= 1000</code></li>
	<li><code>s[i]</code> is either <code>'a'</code> or <code>'b'</code>.</li>
</ul>
</div>